lean-4/GAP2Lean/JsonDecoder.lean
@@ -2,6 +2,7 @@ import Qq
 import GAP2Lean.TreeSet
 import GAP2Lean.TreeMap
 import GAP2Lean.Graph
+import GAP2Lean.Connected
 
 namespace GAP2Lean
 
@@ -30,16 +31,16 @@ def finOfJson (n : Q(Nat)) (j : Lean.Json) : Except String Q(Fin $n) := do
 def vertexOfJson (G : Q(Graph)) (j : Lean.Json) : Except String Q(Graph.vertex $G) := do
   finOfJson (q(Graph.vertexSize $G)) j
 
--- Convert a sub-array into a tree
-partial def from_array {α : Q(Type)} (a : Array Q($α)) (low high : ℕ) : Q(STree $α) :=
+-- Convert a sub-array into a set tree
+partial def stree_from_array {α : Q(Type)} (a : Array Q($α)) (low high : ℕ) : Q(STree $α) :=
   if low >= high then
     q(.empty)
   else if low + 1 = high then
     q(.leaf $(a[low]!))
   else
     let middle := (low + high) / 2
-    let left := from_array a low middle
-    let right := from_array a (middle + 1) high
+    let left := stree_from_array a low middle
+    let right := stree_from_array a (middle + 1) high
     q(.node $(a[middle]!) $left $right)
 
 partial def streeOfJson {α : Q(Type)}
@@ -48,25 +49,32 @@ partial def streeOfJson {α : Q(Type)}
   : Except String Q(STree $α) := do
   let arr ← j.getArr? <|> throw "array expected in streeOfJson"
   let arr ← arr.mapM valOfJson
-  return from_array arr 0 arr.size
+  return stree_from_array arr 0 arr.size
 
-partial def mapTreeOfJson {α β : Q(Type)}
-  (o : Q(Ord $α))
+def pairOfJson (j : Lean.Json) : Except String (Lean.Json × Lean.Json) := do
+  let arr ← j.getArr? <|> throw "pair expected"
+  pure (arr[0]!, arr[1]!)
+
+-- Convert a sub-array into a map tree
+partial def TreeMap_of_array {α β : Q(Type)}
   (keyOfJson : Lean.Json → Except String Q($α))
   (valOfJson : Lean.Json → Except String Q($β))
-  (j : Lean.Json) : Except String Q(Map $α $β) := do
-  let arr ← j.getArr?  <|> throw "array expected in mapTreeOfJson"
-  match arr with
-  | #[] => pure q(Map.empty)
-  | #[k, v] =>
-    pure q(Map.leaf $(← keyOfJson k) $(← valOfJson v))
-  | #[k, v, l, r] =>
+  (arr : Array Lean.Json) (low high : ℕ) : Except String Q(Map $α $β) :=
+  if low >= high then
+    pure q(.empty)
+  else if low + 1 = high then do
+    let (k, v) ← pairOfJson arr[low]!
     let key ← keyOfJson k
     let val ← valOfJson v
-    let left ← mapTreeOfJson o keyOfJson valOfJson l
-    let right ← mapTreeOfJson o keyOfJson valOfJson r
-    pure q(Map.node $key $val $left $right)
-  | _ => throw "invalid tree map format"
+    pure q(.leaf $(key) $(val))
+  else do
+    let middle := (low + high) / 2
+    let left ← TreeMap_of_array keyOfJson valOfJson arr low middle
+    let right ← TreeMap_of_array keyOfJson valOfJson arr (middle + 1) high
+    let (k, v) ← pairOfJson arr[middle]!
+    let key ← keyOfJson k
+    let val ← valOfJson v
+    pure q(.node $(key) $(val) $left $right)
 
 def emptyMap {α β : Type}
   [Decidable (α → False)]
@@ -85,11 +93,11 @@ partial def mapOfJson {α β : Q(Type)}
   | #[] =>
     have H : Q(@Decidable.decide ($α → False) $d = true) := (q(Eq.refl true) : Lean.Expr)
     pure q(emptyMap $H)
-  | #[treeJ, defaultJ] =>
-    let tree ← mapTreeOfJson o keyOfJson valOfJson treeJ
-    let defaultValue ← valOfJson defaultJ
-    pure q(Map.getD $tree $defaultValue)
-  | _ => throw "invalid map format"
+  | arr =>
+    let (_, y) ← pairOfJson arr[0]!
+    let default ← valOfJson y
+    let tree ← TreeMap_of_array keyOfJson valOfJson arr 0 arr.size
+    pure q($(tree).getD $default)
 
 partial def graphOfJson (j : Lean.Json) : Except String Q(Graph) := do
     let vertexSizeJ ← j.getObjVal? "vertexSize"
@@ -98,10 +106,40 @@ partial def graphOfJson (j : Lean.Json) : Except String Q(Graph) := do
       streeOfJson (edgeOfJson vertexSize) (← j.getObjVal? "edges")
     pure q(Graph.mk $vertexSize $edges)
 
+def connectivityCertificateOfJson (G : Q(Graph)) (j : Lean.Json) : Except String Q(ConnectivityCertificate $G) := do
+  let o := q(instOrdFin (Graph.vertexSize $G))
+  let d := q(Fintype.decidableForallFintype)
+  let rootJ ← j.getObjVal? "root"
+  let root ← vertexOfJson G rootJ
+  let nextJ ← j.getObjVal? "next"
+  let next ← mapOfJson o d (vertexOfJson G) (vertexOfJson G) nextJ
+  let distToRootJ ← j.getObjVal? "distToRoot"
+  let distToRoot ← mapOfJson o d (vertexOfJson G) natOfJson distToRootJ
+  have distRootZero : Q(decide ($distToRoot $root = 0) = true) := (q(Eq.refl true) : Lean.Expr)
+  have distZeroRoot : Q(forallVertex (fun (v : Graph.vertex $G) => $distToRoot v = 0 → v = $root) = true) := (q(Eq.refl true) : Lean.Expr)
+  have nextRoot : Q(decide ($next $root = $root) = true) := (q(Eq.refl true) : Lean.Expr)
+  have nextAdjacent : Q(forallVertex (fun v => 0 < $distToRoot v → Graph.adjacent v ($next v)) = true) := (q(Eq.refl true) : Lean.Expr)
+  have distNext : Q(decide (∀ v, 0 < $distToRoot v → $distToRoot ($next v) < $distToRoot v) = true) := (q(Eq.refl true) : Lean.Expr)
+  pure q(@ConnectivityCertificate.mk
+         $G
+         $root
+         $next
+         $distToRoot
+         (of_decide_eq_true $distRootZero)
+         (of_decide_eq_true $distZeroRoot)
+         (of_decide_eq_true $nextRoot)
+         (of_decide_eq_true $nextAdjacent)
+         (of_decide_eq_true $distNext)
+        )
+
 -- lifting from exception monad to the Elab.Command monad
 def liftExcept {α : Type} : Except String α → Lean.Elab.Command.CommandElabM α
   | .ok res => pure res
   | .error msg => throwError msg
+
+-- A name for a cerficicate
+def certificateName (graphName: Lean.Name) (certName: String) : Lean.Name :=
+  (.str graphName certName)
 
 elab "load_graph" graphName:ident fileName:str : command => do
   let graphName := graphName.getId
@@ -119,10 +157,27 @@ elab "load_graph" graphName:ident fileName:str : command => do
     safety := .safe
   }
   Lean.setReducibleAttribute graphName
+  have graph : Q(Graph) := Lean.mkConst graphName []
+  -- load the connectivity certificate
+  let connectivityCertificateName := certificateName graphName "connectivityCertificateI"
+  let connectivityCertificateJ ← liftExcept <| json.getObjVal? "connectivityCertificate"
+  let connectivityCertificateQ : Q(ConnectivityCertificate $graph) ←
+    liftExcept <| connectivityCertificateOfJson graph connectivityCertificateJ
+  Lean.Elab.Command.liftCoreM <| Lean.addAndCompile <| .defnDecl {
+    name := connectivityCertificateName
+    levelParams := []
+    type := q(ConnectivityCertificate $graph)
+    value := connectivityCertificateQ
+    hints := .regular 0
+    safety := .safe
+  }
+  Lean.Elab.Command.liftTermElabM <| Lean.Meta.addInstance connectivityCertificateName .scoped 42
 
-load_graph cow "GAP2Lean/example.json"
 
-#print cow
-#eval cow.adjacent 1 0
+load_graph cow "cert.json"
+
+#check connected_of_certificate cow
+
+
 
 end GAP2Lean
